wip

examples/low-level/crypto/Crypto.Symmetric.Poly1305.Bignum.fst
@@ -21,29 +21,68 @@ module U32 = FStar.UInt32
 module U64 = FStar.UInt64
 module HS = FStar.HyperStack
 
-(* open FStar.Buffer.Quantifiers *)
+open FStar.Buffer.Quantifiers
 
-assume val prime: erased pos
-assume new type willNotOverflow (h:heap) (a_idx:nat) (b_idx:nat) (len:nat) (ctr:nat) (a:bigint) (b:bigint)
-assume new type isNotModified (h0:heap) (h1:heap) (a_idx:nat) (len:nat) (ctr:nat) (a:bigint)
-assume new type isSum (h0:heap) (h1:heap) (a_idx:nat) (b_idx:nat) (len:nat) (ctr:nat) (a:bigint) (b:bigint)
-assume new type satisfiesModuloConstraints (h:heap) (b:bigint)
+val prime: p:erased pos{reveal p = Crypto.Symmetric.Poly1305.Spec.p_1305}
+let prime = hide (Crypto.Symmetric.Poly1305.Spec.p_1305)
+
+let willNotOverflow (h:heap) (a:bigint) (b:bigint) : GTot Type0 =
+  live h a /\ live h b /\ length a >= norm_length /\ length b >= norm_length
+  /\ v (get h a 0) + v (get h b 0) < pow2 64
+  /\ v (get h a 1) + v (get h b 1) < pow2 64
+  /\ v (get h a 2) + v (get h b 2) < pow2 64
+  /\ v (get h a 3) + v (get h b 3) < pow2 64
+  /\ v (get h a 4) + v (get h b 4) < pow2 64
+
+(* assume new type isNotModified (h0:heap) (h1:heap) (a_idx:nat) (len:nat) (ctr:nat) (a:bigint) *)
+
+let isSum (h:heap) (h1:heap) (a:bigint) (b:bigint) : GTot Type0 =
+  live h a /\ live h1 a /\ live h b /\ length a >= norm_length /\ length b >= norm_length
+  /\ v (get h a 0) + v (get h b 0) = v (get h1 a 0)
+  /\ v (get h a 1) + v (get h b 1) = v (get h1 a 1)
+  /\ v (get h a 2) + v (get h b 2) = v (get h1 a 2)
+  /\ v (get h a 3) + v (get h b 3) = v (get h1 a 3)
+  /\ v (get h a 4) + v (get h b 4) = v (get h1 a 4)
+
+
+let bound27 (h:heap) (b:bigint) : GTot Type0 =
+  live h b /\ length b >= norm_length
+  /\ v (get h b 0) < pow2 27
+  /\ v (get h b 1) < pow2 27
+  /\ v (get h b 2) < pow2 27
+  /\ v (get h b 3) < pow2 27
+  /\ v (get h b 4) < pow2 27
+
+(* assume new type satisfiesModuloConstraints (h:heap) (b:bigint) *)
 
 let w : U32.t -> Tot int = U32.v
 
+
 (*** Addition ***)
 
-#reset-options "--z3timeout 20 --initial_fuel 0 --max_fuel 0 --lax"
+#reset-options "--z3timeout 5 --initial_fuel 0 --max_fuel 0"
 
-val fsum': a:bigint -> b:bigint{disjoint a b} -> STL unit
-    (requires (fun h -> norm h a /\ norm h b))
-    (ensures (fun h0 u h1 -> norm h0 a /\ norm h0 b /\ live h1 a
-      /\ modifies_1 a h0 h1
-      /\ eval h1 a norm_length = eval h0 a norm_length + eval h0 b norm_length
-      (* /\ isNotModified h0 h1 0 norm_length 0 a *)
-      (* /\ isSum h0 h1 0 0 norm_length 0 a b *)
-    ))
-let fsum' a b =
+private val lemma_fsum_0:
+  a0:U64.t -> a1:U64.t -> a2:U64.t -> a3:U64.t -> a4:U64.t ->
+  b0:U64.t -> b1:U64.t -> b2:U64.t -> b3:U64.t -> b4:U64.t ->
+  Lemma (requires (let open FStar.UInt64 in
+	  v a0 < pow2 26 /\ v a1 < pow2 26 /\ v a2 < pow2 26 /\ v a3 < pow2 26 /\ v a4 < pow2 26
+	  /\ v b0 < pow2 26 /\ v b1 < pow2 26 /\ v b2 < pow2 26 /\ v b3 < pow2 26 /\ v b4 < pow2 26))
+	(ensures  (let open FStar.UInt64 in
+		  v a0 + v b0 < pow2 64 /\ v a1 + v b1 < pow2 64 /\ v a2 + v b2 < pow2 64
+		  /\ v a3 + v b3 < pow2 64 /\ v a4 + v b4 < pow2 64))
+let lemma_fsum_0 a0 a1 a2 a3 a4 b0 b1 b2 b3 b4 =
+  pow2_double_sum 26;
+  pow2_lt_compat 64 27
+
+
+#reset-options "--z3timeout 20 --initial_fuel 0 --max_fuel 0"
+
+private val fsum_: a:bigint -> b:bigint{disjoint a b} -> STL unit
+  (requires (fun h -> norm h a /\ norm h b))
+  (ensures (fun h0 u h1 -> norm h0 a /\ norm h0 b /\ live h1 a /\ modifies_1 a h0 h1 /\ isSum h0 h1 a b))
+let fsum_ a b =
+  let h0 = HST.get() in
   let a0 = a.(0ul) in
   let a1 = a.(1ul) in
   let a2 = a.(2ul) in
@@ -54,6 +93,11 @@ let fsum' a b =
   let b2 = b.(2ul) in
   let b3 = b.(3ul) in
   let b4 = b.(4ul) in
+  assert(v a0 = v (get h0 a 0)); assert(v a1 = v (get h0 a 1)); assert(v a2 = v (get h0 a 2));
+  assert(v a3 = v (get h0 a 3)); assert(v a4 = v (get h0 a 4)); assert(v b0 = v (get h0 b 0));
+  assert(v b1 = v (get h0 b 1)); assert(v b2 = v (get h0 b 2)); assert(v b3 = v (get h0 b 3));
+  assert(v b4 = v (get h0 b 4));
+  lemma_fsum_0 a0 a1 a2 a3 a4 b0 b1 b2 b3 b4;
   let ab0 = a0 +^ b0 in
   let ab1 = a1 +^ b1 in
   let ab2 = a2 +^ b2 in
@@ -65,50 +109,146 @@ let fsum' a b =
   a.(3ul) <- ab3;
   a.(4ul) <- ab4
 
-  (* let h0 = HST.get() in *)
-  (* cut (pow2 26 + pow2 26 <= pow2 27); *)
-  (* pow2_lt_compat 64 27; *)
-  (* let h0 = HST.get() in *)
-  (* fsum_index a 0ul b 0ul nlength 0ul;  *)
-  (* let h1 = HST.get() in *)
-  (* cut (forall (i:nat). i < norm_length ==> v (get h1 a (i+0)) = v (get h0 a (i+0)) + v (get h0 b (i+0))); *)
-  (* cut (forall (i:nat). (i >= norm_length /\ i < length a) ==> v (get h1 a (i+0)) = v (get h0 a (i+0))); *)
-  (* addition_lemma h0 h1 a b norm_length *)
+assume val lemma_fsum: h0:mem -> h1:mem -> a:bigint -> b:bigint -> Lemma
+  (requires (norm h0 a /\ norm h0 b /\ isSum h0 h1 a b))
+  (ensures  (norm h0 a /\ norm h0 b /\ isSum h0 h1 a b
+    /\ bound27 h1 a /\ eval h1 a norm_length = eval h0 a norm_length + eval h0 b norm_length))
 
-val scalar_multiplication: res:bigint -> a:bigint{disjoint res a} -> s:u64 -> Stack unit
-  (requires (fun h -> live h res /\ live h a
-    (* /\ (forall (i:nat). {:pattern (v (get h a i))} i < norm_length ==> v (get h a i) * v s < pow2 64)  *)
-  ))
-  (ensures (fun h0 _ h1 -> live h1 res /\ modifies_1 res h0 h1
-    (* /\ scalarProduct h0 h1 norm_length a s res *)
-    (* /\ equal h0 a h1 a *)
-    (* /\ equalSub h0 res norm_length h1 res norm_length (length res - norm_length) *)
-    (* /\ eval h1 res norm_length = eval h0 a norm_length * v s *)
-  ))
-let scalar_multiplication res a s =
-  let a0 = a.(0ul) in
-  let a1 = a.(1ul) in
-  let a2 = a.(2ul) in
-  let a3 = a.(3ul) in
-  let a4 = a.(4ul) in
-  a.(0ul) <- a0 *^ s;
-  a.(1ul) <- a1 *^ s;
-  a.(2ul) <- a2 *^ s;
-  a.(3ul) <- a3 *^ s;
-  a.(4ul) <- a4 *^ s
+val fsum': a:bigint -> b:bigint{disjoint a b} -> STL unit
+    (requires (fun h -> norm h a /\ norm h b))
+    (ensures (fun h0 u h1 -> norm h0 a /\ norm h0 b /\ bound27 h1 a /\ modifies_1 a h0 h1
+      /\ eval h1 a norm_length = eval h0 a norm_length + eval h0 b norm_length
+    ))
+let fsum' a b =
+  let h0 = HST.get() in
+  fsum_ a b;
+  let h1 = HST.get() in
+  lemma_fsum h0 h1 a b
 
-assume new type bound27 (h:mem) (a:bigint)
+#reset-options "--z3timeout 20 --initial_fuel 0 --max_fuel 0"
 
-val multiplication: c:bigint -> a:bigint{disjoint c a} -> b:bigint{disjoint c b} -> Stack unit
-     (requires (fun h -> bound27 h a /\ norm h b /\ live h c /\ null h c))
-     (ensures (fun h0 u h1 -> bound27 h0 a /\ norm h0 b /\ live h1 c
-       /\ modifies_1 c h0 h1
-       (* /\ eval h1 c (2*norm_length-1) = eval h0 a (norm_length) * eval h0 b (norm_length) *)
-       (* /\ maxValue h1 c (length c) <= norm_length * pow2 53 *)
-     ))
-let multiplication c a b =
-  let a0 = a.(0ul) in let a1 = a.(1ul) in let a2 = a.(2ul) in let a3 = a.(3ul) in let a4 = a.(4ul) in
-  let b0 = b.(0ul) in let b1 = b.(1ul) in let b2 = b.(2ul) in let b3 = b.(3ul) in let b4 = b.(4ul) in
+let isMultiplication (h0:mem) (h1:mem) (a:bigint) (b:bigint) (c:bigint) : GTot Type0 =
+  live h0 a /\ live h0 b /\ live h1 c
+  /\ length a >= norm_length /\ length b >= norm_length /\ length c >= 2*norm_length-1
+  /\ (
+    let a0 = v (get h0 a 0) in let a1 = v (get h0 a 1) in let a2 = v (get h0 a 2) in
+    let a3 = v (get h0 a 3) in let a4 = v (get h0 a 4) in let b0 = v (get h0 b 0) in
+    let b1 = v (get h0 b 1) in let b2 = v (get h0 b 2) in let b3 = v (get h0 b 3) in
+    let b4 = v (get h0 b 4) in let c0 = v (get h1 c 0) in let c1 = v (get h1 c 1) in
+    let c2 = v (get h1 c 2) in let c3 = v (get h1 c 3) in let c4 = v (get h1 c 4) in
+    let c5 = v (get h1 c 5) in let c6 = v (get h1 c 6) in let c7 = v (get h1 c 7) in
+    let c8 = v (get h1 c 8) in
+    ( c1 = a0 * b1 + a1 * b0
+      /\ c2 = a0 * b2 + a1 * b1 + a2 * b0
+      /\ c3 = a0 * b3 + a1 * b2 + a2 * b1 + a3 * b0
+      /\ c4 = a0 * b4 + a1 * b3 + a2 * b2 + a3 * b1 + a4 * b0
+      /\ c5 = a1 * b4 + a2 * b3 + a3 * b2 + a4 * b1
+      /\ c6 = a2 * b4 + a3 * b3 + a4 * b2
+      /\ c7 = a3 * b4 + a4 * b3
+      /\ c8 = a4 * b4 ) )
+
+private let isMultiplication_
+  (h1:mem)
+  (a0:int) (a1:int) (a2:int) (a3:int) (a4:int)
+  (b0:int) (b1:int) (b2:int) (b3:int) (b4:int)
+  (c:bigint) : GTot Type0 =
+  live h1 c /\ length c >= 2*norm_length-1
+  /\ (
+      let c0 = v (get h1 c 0) in let c1 = v (get h1 c 1) in
+      let c2 = v (get h1 c 2) in let c3 = v (get h1 c 3) in let c4 = v (get h1 c 4) in
+      let c5 = v (get h1 c 5) in let c6 = v (get h1 c 6) in let c7 = v (get h1 c 7) in
+      let c8 = v (get h1 c 8) in
+      ( c1 = a0 * b1 + a1 * b0
+	/\ c2 = a0 * b2 + a1 * b1 + a2 * b0
+	/\ c3 = a0 * b3 + a1 * b2 + a2 * b1 + a3 * b0
+	/\ c4 = a0 * b4 + a1 * b3 + a2 * b2 + a3 * b1 + a4 * b0
+	/\ c5 = a1 * b4 + a2 * b3 + a3 * b2 + a4 * b1
+	/\ c6 = a2 * b4 + a3 * b3 + a4 * b2
+	/\ c7 = a3 * b4 + a4 * b3
+	/\ c8 = a4 * b4 ) )
+
+private val lemma_multiplication_0:
+  a0:U64.t -> a1:U64.t -> a2:U64.t -> a3:U64.t -> a4:U64.t ->
+  b0:U64.t -> b1:U64.t -> b2:U64.t -> b3:U64.t -> b4:U64.t ->
+  Lemma (requires (let open FStar.UInt64 in
+	  v a0 < pow2 27 /\ v a1 < pow2 27 /\ v a2 < pow2 27 /\ v a3 < pow2 27 /\ v a4 < pow2 27
+	  /\ v b0 < pow2 26 /\ v b1 < pow2 26 /\ v b2 < pow2 26 /\ v b3 < pow2 26 /\ v b4 < pow2 26))
+	(ensures  (let open FStar.UInt64 in
+	  v a0 * v b0 < pow2 64 /\ v a1 * v b0 < pow2 64 /\ v a2 * v b0 < pow2 64
+	  /\ v a3 * v b0 < pow2 64 /\ v a4 * v b0 < pow2 64 /\ v a0 * v b1 < pow2 64
+	  /\ v a1 * v b1 < pow2 64 /\ v a2 * v b1 < pow2 64 /\ v a3 * v b1 < pow2 64
+	  /\ v a4 * v b1 < pow2 64 /\ v a0 * v b2 < pow2 64 /\ v a1 * v b2 < pow2 64
+	  /\ v a2 * v b2 < pow2 64 /\ v a3 * v b2 < pow2 64 /\ v a4 * v b2 < pow2 64
+	  /\ v a0 * v b3 < pow2 64 /\ v a1 * v b3 < pow2 64 /\ v a2 * v b3 < pow2 64
+	  /\ v a3 * v b3 < pow2 64 /\ v a4 * v b3 < pow2 64 /\ v a0 * v b4 < pow2 64
+	  /\ v a1 * v b4 < pow2 64 /\ v a2 * v b4 < pow2 64 /\ v a3 * v b4 < pow2 64
+	  /\ v a4 * v b4 < pow2 64
+	  /\ v a0 * v b1 + v a1 * v b0 < pow2 64
+	  /\ v a0 * v b2 + v a1 * v b1 < pow2 64
+	  /\ v a0 * v b2 + v a1 * v b1 + v a2 * v b0 < pow2 64
+	  /\ v a0 * v b3 + v a1 * v b2 < pow2 64
+	  /\ v a0 * v b3 + v a1 * v b2 + v a2 * v b1 < pow2 64
+	  /\ v a0 * v b3 + v a1 * v b2 + v a2 * v b1 + v a3 * v b0 < pow2 64
+	  /\ v a0 * v b4 + v a1 * v b3 < pow2 64
+	  /\ v a0 * v b4 + v a1 * v b3 + v a2 * v b2 < pow2 64
+	  /\ v a0 * v b4 + v a1 * v b3 + v a2 * v b2 + v a3 * v b1 < pow2 64
+	  /\ v a0 * v b4 + v a1 * v b3 + v a2 * v b2 + v a3 * v b1 + v a4 * v b0 < pow2 64
+	  /\ v a1 * v b4 + v a2 * v b3 < pow2 64
+	  /\ v a1 * v b4 + v a2 * v b3 + v a3 * v b2 < pow2 64
+	  /\ v a1 * v b4 + v a2 * v b3 + v a3 * v b2 + v a4 * v b1 < pow2 64
+	  /\ v a2 * v b4 + v a3 * v b3 < pow2 64
+	  /\ v a2 * v b4 + v a3 * v b3 + v a4 * v b2 < pow2 64
+	  /\ v a3 * v b4 + v a4 * v b3 < pow2 64
+	  ))
+let lemma_multiplication_0 a0 a1 a2 a3 a4 b0 b1 b2 b3 b4 =
+  assert(forall (a:nat) (b:nat) c d. {:pattern (a * b); (c * d)} (a < c /\ b < d) ==> a * b < c * d);
+  pow2_plus 27 26;
+  pow2_lt_compat 64 53;
+  pow2_double_sum 53;
+  pow2_lt_compat 64 54;
+  pow2_double_sum 54;
+  pow2_lt_compat 64 55;
+  pow2_double_sum 55;
+  pow2_lt_compat 64 56
+
+#reset-options "--z3timeout 20 --initial_fuel 0 --max_fuel 0"
+
+let u27 = x:FStar.UInt64.t{v x < pow2 27}
+let u26 = x:FStar.UInt64.t{v x < pow2 26}
+
+private val update_9: c:bigint{length c >= 2*norm_length-1} ->
+  c0:U64.t -> c1:U64.t -> c2:U64.t ->
+  c3:U64.t -> c4:U64.t -> c5:U64.t ->
+  c6:U64.t -> c7:U64.t -> c8:U64.t ->
+  Stack unit
+    (requires (fun h -> live h c))
+    (ensures  (fun h0 _ h1 -> live h1 c /\ modifies_1 c h0 h1
+      /\ get h1 c 0 == c0 /\ get h1 c 1 == c1 /\ get h1 c 2 == c2
+      /\ get h1 c 3 == c3 /\ get h1 c 4 == c4 /\ get h1 c 5 == c5
+      /\ get h1 c 6 == c6 /\ get h1 c 7 == c7 /\ get h1 c 8 == c8))
+let update_9 c c0 c1 c2 c3 c4 c5 c6 c7 c8 =
+  c.(0ul) <- c0;
+  c.(1ul) <- c1;
+  c.(2ul) <- c2;
+  c.(3ul) <- c3;
+  c.(4ul) <- c4;
+  c.(5ul) <- c5;
+  c.(6ul) <- c6;
+  c.(7ul) <- c7;
+  c.(8ul) <- c8
+
+#reset-options "--z3timeout 20 --initial_fuel 0 --max_fuel 0"
+
+private val multiplication_0:
+  c:bigint{length c >= 2*norm_length-1} ->
+  a0:u27 -> a1:u27 -> a2:u27 -> a3:u27 -> a4:u27 ->
+  b0:u26 -> b1:u26 -> b2:u26 -> b3:u26 -> b4:u26 ->
+  Stack unit
+    (requires (fun h -> live h c))
+    (ensures  (fun h0 _ h1 -> modifies_1 c h0 h1 /\ live h1 c
+      /\ isMultiplication_ h1 (v a0) (v a1) (v a2) (v a3) (v a4) (v b0) (v b1) (v b2) (v b3) (v b4) c))
+let multiplication_0 c a0 a1 a2 a3 a4 b0 b1 b2 b3 b4 =
+  lemma_multiplication_0 a0 a1 a2 a3 a4 b0 b1 b2 b3 b4;
   let ab00 = a0 *^ b0 in
   let ab01 = a0 *^ b1 in
   let ab02 = a0 *^ b2 in
@@ -143,30 +283,97 @@ let multiplication c a b =
   let c6 = ab24 +^ ab33 +^ ab42 in
   let c7 = ab34 +^ ab43 in
   let c8 = ab44 in
-  c.(0ul) <- c0;
-  c.(1ul) <- c1;
-  c.(2ul) <- c2;
-  c.(3ul) <- c3;
-  c.(4ul) <- c4;
-  c.(5ul) <- c5;
-  c.(6ul) <- c6;
-  c.(7ul) <- c7;
-  c.(8ul) <- c8
+  update_9 c c0 c1 c2 c3 c4 c5 c6 c7 c8
 
-val times_5: b:U64.t -> Tot (b':U64.t)
+private val multiplication_:
+  c:bigint{length c >= 2 * norm_length - 1} ->
+  a:bigint{disjoint c a} ->
+  b:bigint{disjoint c b} ->
+  Stack unit
+     (requires (fun h -> bound27 h a /\ norm h b /\ live h c))
+     (ensures (fun h0 u h1 -> bound27 h0 a /\ norm h0 b /\ live h1 c /\ modifies_1 c h0 h1
+       /\ isMultiplication h0 h1 a b c
+     ))
+let multiplication_ c a b =
+  let h0 = HST.get() in
+  let a0 = a.(0ul) in let a1 = a.(1ul) in let a2 = a.(2ul) in let a3 = a.(3ul) in let a4 = a.(4ul) in
+  let b0 = b.(0ul) in let b1 = b.(1ul) in let b2 = b.(2ul) in let b3 = b.(3ul) in let b4 = b.(4ul) in
+  multiplication_0 c a0 a1 a2 a3 a4 b0 b1 b2 b3 b4
+
+assume val lemma_multiplication:
+  h0:mem ->
+  h1:mem ->
+  c:bigint{length c >= 2*norm_length-1} ->
+  a:bigint{disjoint c a} ->
+  b:bigint{disjoint c b} ->
+  Lemma (requires (bound27 h0 a /\ norm h0 b /\ live h1 c /\ isMultiplication h0 h1 a b c))
+	(ensures  (bound27 h0 a /\ norm h0 b /\ live h1 c /\ isMultiplication h0 h1 a b c
+	  /\ eval h1 c (2*norm_length-1) = eval h0 a norm_length * eval h0 b norm_length
+	  /\ maxValue h1 c (2*norm_length-1) <= norm_length * pow2 53))
+
+val multiplication:
+  c:bigint{length c >= 2 * norm_length - 1} ->
+  a:bigint{disjoint c a} ->
+  b:bigint{disjoint c b} ->
+  Stack unit
+     (requires (fun h -> bound27 h a /\ norm h b /\ live h c))
+     (ensures (fun h0 u h1 -> bound27 h0 a /\ norm h0 b /\ live h1 c /\ modifies_1 c h0 h1
+       /\ eval h1 c (2*norm_length-1) = eval h0 a (norm_length) * eval h0 b (norm_length)
+       /\ maxValue h1 c (2*norm_length-1) <= norm_length * pow2 53
+     ))
+let multiplication c a b =
+  let h0 = HST.get() in
+  multiplication_ c a b;
+  let h1 = HST.get() in
+  lemma_multiplication h0 h1 c a b
+
+
+#reset-options "--z3timeout 5 --initial_fuel 3 --max_fuel 3"
+
+val times_5: b:U64.t{5 * v b < pow2 64} -> Tot (b':U64.t{v b' = 5 * v b})
 let times_5 b = (b <<^ 2ul) +^ b
 
-val freduce_degree: b:bigint -> Stack unit
-  (requires (fun h -> live h b
-    (* /\ satisfiesModuloConstraints h b *)
-  ))
+#reset-options "--z3timeout 5 --initial_fuel 0 --max_fuel 0"
+
+let isDegreeReduced (h0:mem) (h1:mem) (b:bigint) =
+  live h0 b /\ live h1 b /\ length b >= 2*norm_length-1
+  /\ v (get h1 b 0) = v (get h0 b 0) + 5 * v (get h0 b 5)
+  /\ v (get h1 b 1) = v (get h0 b 1) + 5 * v (get h0 b 6)
+  /\ v (get h1 b 2) = v (get h0 b 2) + 5 * v (get h0 b 7)
+  /\ v (get h1 b 3) = v (get h0 b 3) + 5 * v (get h0 b 8)
+
+let satisfiesModuloConstraints (h:heap) (b:bigint) : GTot Type0 =
+  live h b /\ length b >= 2*norm_length-1
+  /\ maxValue h b (2*norm_length-1) * 6 < pow2 63
+
+private val lemma_freduce_degree_0:
+  h:mem ->
+  b:bigint ->
+  Lemma (requires (satisfiesModuloConstraints h b))
+	(ensures  (satisfiesModuloConstraints h b
+	  /\ 5 * v (get h b 5) < pow2 64 /\ 5 * v (get h b 6) < pow2 64 /\ 5 * v (get h b 7) < pow2 64
+	  /\ 5 * v (get h b 7) < pow2 64 /\ 5 * v (get h b 8) < pow2 64
+	  /\ v (get h b 0) + 5 * v (get h b 5) < pow2 64 /\ v (get h b 1) + 5 * v (get h b 6) < pow2 64
+	  /\ v (get h b 2) + 5 * v (get h b 7) < pow2 64 /\ v (get h b 3) + 5 * v (get h b 8) < pow2 64
+	))
+let lemma_freduce_degree_0 h b =
+  pow2_double_sum 63;
+  maxValue_lemma_aux h b (2*norm_length-1)
+
+
+#reset-options "--z3timeout 20 --initial_fuel 0 --max_fuel 0"
+
+val freduce_degree_: b:bigint -> Stack unit
+  (requires (fun h -> live h b /\ satisfiesModuloConstraints h b))
   (ensures (fun h0 _ h1 -> live h0 b /\ live h1 b /\ modifies_1 b h0 h1
+    /\ isDegreeReduced h0 h1 b
     (* /\ satisfiesModuloConstraints h0 b *)
     (* /\ (forall (i:nat). {:pattern (v (get h1 b i))} i <= norm_length ==> *)
     (* 	v (get h1 b i) < pow2 63) *)
     (* /\ eval h1 b norm_length % reveal prime = eval h0 b (2*norm_length-1) % reveal prime *)
   ))
-let freduce_degree b =
+let freduce_degree_ b =
+  let h0 = HST.get() in
   let b0 = b.(0ul) in
   let b1 = b.(1ul) in
   let b2 = b.(2ul) in
@@ -175,6 +382,7 @@ let freduce_degree b =
   let b6 = b.(6ul) in
   let b7 = b.(7ul) in
   let b8 = b.(8ul) in
+  lemma_freduce_degree_0 h0 b;
   let b0' = b0 +^ times_5 b5 in
   let b1' = b1 +^ times_5 b6 in
   let b2' = b2 +^ times_5 b7 in
@@ -184,25 +392,136 @@ let freduce_degree b =
   b.(2ul) <- b2';
   b.(3ul) <- b3'
 
-val mod2_26: U64.t -> Tot U64.t
-let mod2_26 x = x &^ 0x3ffffffuL
+let bound63 (h:heap) (b:bigint) : GTot Type0 =
+  live h b /\ v (get h b 0) < pow2 63 /\ v (get h b 1) < pow2 63 /\ v (get h b 2) < pow2 63
+  /\ v (get h b 3) < pow2 63 /\ v (get h b 4) < pow2 63
 
-val div2_26: U64.t -> Tot U64.t
-let div2_26 x = x >>^ 26ul
+assume val lemma_freduce_degree:
+  h0:mem ->
+  h1:mem ->
+  b:bigint ->
+  Lemma (requires (satisfiesModuloConstraints h0 b /\ isDegreeReduced h0 h1 b))
+	(ensures  (satisfiesModuloConstraints h0 b /\ isDegreeReduced h0 h1 b
+	  /\ bound63 h1 b
+	  /\ eval h1 b norm_length % reveal prime = eval h0 b (2*norm_length-1) % reveal prime))
 
-val carry_1: b:bigint -> Stack unit
-  (requires (fun h -> live h b
-    (* /\ (forall (i:nat). {:pattern (v (get h b i))} i < norm_length ==> v (get h b i) < pow2 63) *)
+
+val freduce_degree: b:bigint -> Stack unit
+  (requires (fun h -> satisfiesModuloConstraints h b))
+  (ensures (fun h0 _ h1 -> live h0 b /\ live h1 b /\ modifies_1 b h0 h1
+    /\ satisfiesModuloConstraints h0 b
+    /\ bound63 h1 b
+    /\ eval h1 b norm_length % reveal prime = eval h0 b (2*norm_length-1) % reveal prime
   ))
-  (ensures (fun h0 _ h1 -> live h0 b /\ norm h1 b /\ modifies_1 b h0 h1
+let freduce_degree b =
+  let h0 = HST.get() in
+  freduce_degree_ b;
+  let h1 = HST.get() in
+  lemma_freduce_degree h0 h1 b
+
+private val mod2_26: x:U64.t -> Tot (y:U64.t{v y = v x % pow2 26 /\ v y < pow2 26})
+let mod2_26 x =
+  let y = x &^ 0x3ffffffuL in
+  assume (v y = v x % pow2 26);
+  y
+
+private val div2_26: x:U64.t -> Tot (y:U64.t{v y = v x / pow2 26 /\ v y <= pow2 38})
+let div2_26 x = pow2_minus 64 26; x >>^ 26ul
+
+#reset-options "--z3timeout 20 --initial_fuel 0 --max_fuel 0"
+
+let isCarried (h0:mem) (h1:mem) (b:bigint) : GTot Type0 =
+  live h0 b /\ live h1 b /\ length b >= norm_length+1
+  /\ (
+      let b0 = v (get h0 b 0) in
+      let b1 = v (get h0 b 1) in
+      let b2 = v (get h0 b 2) in
+      let b3 = v (get h0 b 3) in
+      let b4 = v (get h0 b 4) in
+      let r0  = b0 / pow2 26 in
+      let r1  = (b1 + r0) / pow2 26 in
+      let r2  = (b2 + r1) / pow2 26 in
+      let r3  = (b3 + r2) / pow2 26 in
+      v (get h1 b 0) = b0 % pow2 26
+      /\ v (get h1 b 1) = (b1 + r0)  % pow2 26
+      /\ v (get h1 b 2) = (b2 + r1)  % pow2 26
+      /\ v (get h1 b 3) = (b3 + r2)  % pow2 26
+      /\ v (get h1 b 4) = (b4 + r3)  % pow2 26
+      /\ length b >= 6
+      /\ v (get h1 b 5) = (b4 + r3) / pow2 26
+    )
+
+private val update_5: c:bigint ->
+  c0:U64.t -> c1:U64.t -> c2:U64.t ->
+  c3:U64.t -> c4:U64.t ->
+  Stack unit
+    (requires (fun h -> live h c))
+    (ensures  (fun h0 _ h1 -> live h1 c /\ modifies_1 c h0 h1
+      /\ get h1 c 0 == c0 /\ get h1 c 1 == c1 /\ get h1 c 2 == c2
+      /\ get h1 c 3 == c3 /\ get h1 c 4 == c4))
+let update_5 c c0 c1 c2 c3 c4 =
+  c.(0ul) <- c0;
+  c.(1ul) <- c1;
+  c.(2ul) <- c2;
+  c.(3ul) <- c3;
+  c.(4ul) <- c4
+
+#reset-options "--z3timeout 20 --initial_fuel 0 --max_fuel 0"
+
+private val update_6: c:bigint{length c >= norm_length+1} ->
+  c0:U64.t -> c1:U64.t -> c2:U64.t ->
+  c3:U64.t -> c4:U64.t -> c5:U64.t ->
+  Stack unit
+    (requires (fun h -> live h c))
+    (ensures  (fun h0 _ h1 -> live h1 c /\ modifies_1 c h0 h1
+      /\ get h1 c 0 == c0 /\ get h1 c 1 == c1 /\ get h1 c 2 == c2
+      /\ get h1 c 3 == c3 /\ get h1 c 4 == c4 /\ get h1 c 5 == c5))
+let update_6 c c0 c1 c2 c3 c4 c5  =
+  c.(0ul) <- c0;
+  c.(1ul) <- c1;
+  c.(2ul) <- c2;
+  c.(3ul) <- c3;
+  c.(4ul) <- c4;
+  c.(5ul) <- c5
+
+#reset-options "--z3timeout 20 --initial_fuel 0 --max_fuel 0"
+
+
+let u633 = x:U64.t{v x < pow2 63}
+
+
+let isCarried_
+  (h1:mem)
+  (b0:U64.t) (b1:U64.t) (b2:U64.t) (b3:U64.t) (b4:U64.t)
+  (b:bigint) : GTot Type0 =
+  live h1 b /\ length b >= norm_length+1
+  /\ (
+      let r0  = v b0 / pow2 26 in
+      let r1  = (v b1 + r0) / pow2 26 in
+      let r2  = (v b2 + r1) / pow2 26 in
+      let r3  = (v b3 + r2) / pow2 26 in
+      v (get h1 b 0) = v b0 % pow2 26
+      /\ v (get h1 b 1) = (v b1 + r0)  % pow2 26
+      /\ v (get h1 b 2) = (v b2 + r1)  % pow2 26
+      /\ v (get h1 b 3) = (v b3 + r2)  % pow2 26
+      /\ v (get h1 b 4) = (v b4 + r3)  % pow2 26
+      /\ v (get h1 b 5) = (v b4 + r3) / pow2 26
+    )
+
+
+private val carry_1_0:
+  b:bigint{length b >= norm_length+1} ->
+  b0:u633 -> b1:u633 -> b2:u633 -> b3:u633 -> b4:u633 ->
+  Stack unit
+    (requires (fun h -> bound63 h b))
+    (ensures (fun h0 _ h1 -> bound63 h0 b /\ norm h1 b /\ modifies_1 b h0 h1
+      /\ isCarried_ h1 b0 b1 b2 b3 b4 b
     (* /\ eval h1 b norm_length % reveal prime = eval h0 b norm_length % reveal prime *)
-  ))
-let carry_1 b =
-  let b0 = b.(0ul) in
-  let b1 = b.(1ul) in
-  let b2 = b.(2ul) in
-  let b3 = b.(3ul) in
-  let b4 = b.(4ul) in
+    ))
+let carry_1_0 b b0 b1 b2 b3 b4 =
+  pow2_lt_compat 39 38; pow2_lt_compat 63 39; pow2_double_sum 63;
+  assert(forall x y. {:pattern (v x + v y)}(v x < pow2 63 /\ v y <= pow2 38)
+    ==> v x + v y < pow2 64);
   let b0' = mod2_26 b0 in
   let r0  = div2_26 b0 in
   let b1' = mod2_26 (b1 +^ r0) in
@@ -213,43 +532,94 @@ let carry_1 b =
   let r3  = div2_26 (b3 +^ r2) in
   let b4' = mod2_26 (b4 +^ r3) in
   let b5' = div2_26 (b4 +^ r3) in
-  b.(0ul) <- b0';
-  b.(1ul) <- b1';
-  b.(2ul) <- b2';
-  b.(3ul) <- b3';
-  b.(4ul) <- b4';
-  b.(5ul) <- b5'
+  update_6 b b0' b1' b2' b3' b4' b5'
 
+
+#reset-options "--z3timeout 20 --initial_fuel 0 --max_fuel 0"
+
+private val carry_1_:
+  b:bigint{length b >= norm_length+1} ->
+  Stack unit
+    (requires (fun h -> bound63 h b))
+    (ensures (fun h0 _ h1 -> bound63 h0 b /\ norm h1 b /\ modifies_1 b h0 h1
+      /\ isCarried h0 h1 b
+    (* /\ eval h1 b norm_length % reveal prime = eval h0 b norm_length % reveal prime *)
+    ))
+let carry_1_ b =
+  let b0 = b.(0ul) in
+  let b1 = b.(1ul) in
+  let b2 = b.(2ul) in
+  let b3 = b.(3ul) in
+  let b4 = b.(4ul) in
+  carry_1_0 b b0 b1 b2 b3 b4
+
+let carried_1 (h:mem) (b:bigint) : GTot Type0 =
+  live h b /\ length b >= norm_length+1
+  /\ v (get h b 0) < pow2 26
+  /\ v (get h b 1) < pow2 26
+  /\ v (get h b 2) < pow2 26
+  /\ v (get h b 3) < pow2 26
+  /\ v (get h b 4) < pow2 26
+  /\ v (get h b 5) <= pow2 38
+
+assume val lemma_carry_1:
+  h0:mem -> h1:mem ->
+  b:bigint{length b >= norm_length+1} ->
+  Lemma (requires (bound63 h0 b /\ isCarried h0 h1 b))
+	(ensures  (bound63 h0 b /\ isCarried h0 h1 b
+	  /\ eval h1 b (norm_length+1) = eval h0 b norm_length /\ carried_1 h1 b))
+
+val carry_1:
+  b:bigint{length b >= norm_length+1} ->
+  Stack unit
+    (requires (fun h -> bound63 h b))
+    (ensures (fun h0 _ h1 -> bound63 h0 b /\ norm h1 b /\ modifies_1 b h0 h1
+      /\ eval h1 b (norm_length+1) = eval h0 b norm_length /\ carried_1 h1 b
+    ))
+let carry_1 b =
+  let h0 = HST.get() in
+  carry_1_ b;
+  let h1 = HST.get() in
+  lemma_carry_1 h0 h1 b
+
+
+let carried_2 (h:mem) (b:bigint) : GTot Type0 =
+  live h b /\ length b >= norm_length+1
+  /\ v (get h b 0) < pow2 42
+  /\ v (get h b 1) < pow2 26
+  /\ v (get h b 2) < pow2 26
+  /\ v (get h b 3) < pow2 26
+  /\ v (get h b 4) < pow2 26
+
+val carry_2_: b:bigint -> Stack unit
+  (requires (fun h -> carried_2 h b))
+  (ensures (fun h0 _ h1 -> live h0 b /\ norm h1 b /\ modifies_1 b h0 h1
+    /\ isCarried h0 h1 b
+    (* /\ eval h1 b norm_length % reveal prime = eval h0 b norm_length % reveal prime *)
+  ))
+let carry_2_ b =
+  pow2_lt_compat 63 42; pow2_lt_compat 63 26;
+  carry_1_ b
+
+assume val lemma_carry_2:
+  h0:mem -> h1:mem ->
+  b:bigint{length b >= norm_length+1} ->
+  Lemma (requires (carried_2 h0 b /\ isCarried h0 h1 b))
+	(ensures  (carried_2 h0 b /\ isCarried h0 h1 b
+	  /\ eval h1 b (norm_length+1) = eval h0 b norm_length
+	  /\ norm h1 b))
 
 val carry_2: b:bigint -> Stack unit
-  (requires (fun h -> live h b
-    (* /\ (forall (i:nat). {:pattern (v (get h b i))} i < norm_length ==> v (get h b i) < pow2 63) *)
-  ))
+  (requires (fun h -> carried_2 h b))
   (ensures (fun h0 _ h1 -> live h0 b /\ norm h1 b /\ modifies_1 b h0 h1
-    (* /\ eval h1 b norm_length % reveal prime = eval h0 b norm_length % reveal prime *)
+	  /\ eval h1 b (norm_length+1) = eval h0 b norm_length
+	  /\ norm h1 b
   ))
 let carry_2 b =
-  let b0 = b.(0ul) in
-  let b1 = b.(1ul) in
-  let b2 = b.(2ul) in
-  let b3 = b.(3ul) in
-  let b4 = b.(4ul) in
-  let b0' = mod2_26 b0 in
-  let r0  = div2_26 b0 in
-  let b1' = mod2_26 (b1 +^ r0) in
-  let r1  = div2_26 (b1 +^ r0) in
-  let b2' = mod2_26 (b2 +^ r1) in
-  let r2  = div2_26 (b2 +^ r1) in
-  let b3' = mod2_26 (b3 +^ r2) in
-  let r3  = div2_26 (b3 +^ r2) in
-  let b4' = mod2_26 (b4 +^ r3) in
-  let b5' = div2_26 (b4 +^ r3) in
-  b.(0ul) <- b0';
-  b.(1ul) <- b1';
-  b.(2ul) <- b2';
-  b.(3ul) <- b3';
-  b.(4ul) <- b4';
-  b.(5ul) <- b5'
+  let h0 = HST.get() in
+  carry_2_ b;
+  let h1 = HST.get() in
+  lemma_carry_2 h0 h1 b
 
 val carry_top: b:bigint -> Stack unit
   (requires (fun h -> live h b /\ length b >= 5))
